theories/sim/body.v
@@ -44,9 +44,10 @@ Proof.
   intros. eapply HΦ; done.
 Qed.
 
-Lemma sim_body_bind fs ft r n
-  (Ks: list (ectxi_language.ectx_item (bor_ectxi_lang fs)))
-  (Kt: list (ectxi_language.ectx_item (bor_ectxi_lang ft))) es et σs σt Φ :
+Lemma sim_body_bind fs ft
+  (Ks: list (ectxi_language.ectx_item (bor_ectxi_lang fs))) es
+  (Kt: list (ectxi_language.ectx_item (bor_ectxi_lang ft))) et
+  r n σs σt Φ :
   r ⊨{n,fs,ft} (es, σs) ≥ (et, σt)
     : (λ r' n' es' σs' et' σt',
         r' ⊨{n',fs,ft} (fill Ks es', σs') ≥ (fill Kt et', σt') : Φ) →
@@ -131,6 +132,26 @@ Proof.
     exists idx'. rewrite 2!fill_app.
     pclearbot. right. by apply CIH. }
 Qed.
+
+Lemma sim_body_bind_r fs ft
+  (Kt: list (ectxi_language.ectx_item (bor_ectxi_lang ft))) et
+  r n es σs σt Φ :
+  r ⊨{n,fs,ft} (#[], σs) ≥ (et, σt)
+    : (λ r' n' _ _ et' σt',
+        r' ⊨{n',fs,ft} (es, σs) ≥ (fill Kt et', σt') : Φ) →
+  r ⊨{n,fs,ft} (es, σs) ≥ (fill Kt et, σt) : Φ.
+Proof.
+Admitted.
+
+Lemma sim_body_bind_l fs ft
+  (Ks: list (ectxi_language.ectx_item (bor_ectxi_lang ft))) es
+  r n et σs σt Φ :
+  r ⊨{n,fs,ft} (es, σs) ≥ (#[], σt)
+    : (λ r' n' es' σs' _ _,
+        r' ⊨{n',fs,ft} (fill Ks es', σs') ≥ (et, σt) : Φ) →
+  r ⊨{n,fs,ft} (fill Ks es, σs) ≥ (et, σt) : Φ.
+Proof.
+Admitted.
 
 Lemma sim_body_bind_call r n fs ft es σs et σt (fns fnt: result) (pres pret: list result) posts postt Φ :
   r ⊨{n,fs,ft} (es, σs) ≥ (et, σt)
