theories/sim/right_step.v
@@ -5,13 +5,42 @@ From stbor.sim Require Export instance.
 
 Set Default Proof Using "Type".
 
-Lemma sim_body_copy_right_1
-  fs ft (r: resUR) k (h: heapletR) n l t s es σs σt Φ
-  (* we know we're going to read s *)
-  (UNIQUE: r.(rtm) !! t ≡ Some (k, h))
-  (InD: h !! l ≡ Some (to_agree s))
-  (IN: tag_in_stack σt l t) :
-  (σt.(shp) !! l = Some s → r ⊨{n,fs,ft} (es, σs) ≥ (#[s%S], σt) : Φ : Prop) →
-  r ⊨{n,fs,ft} (es, σs) ≥ (Copy (Place l (Tagged t) int), σt) : Φ.
+Section right.
+Implicit Types Φ: resUR → nat → result → state → result → state → Prop.
+
+Lemma sim_body_let_r fs ft r n x es et1 et2 vt1 σs σt Φ :
+  IntoResult et1 vt1 →
+  r ⊨{n,fs,ft} (es, σs) ≥ (subst' x et1 et2, σt) : Φ →
+  r ⊨{S n,fs,ft} (es, σs) ≥ (let: x := et1 in et2, σt) : Φ.
 Proof.
-Abort.
+Admitted.
+
+Lemma sim_body_deref_r fs ft r n es (rs: result) l t T σs σt Φ :
+  IntoResult es rs →
+  (Φ r n rs σs (PlaceR l t T) σt) →
+  r ⊨{S n,fs,ft} (es, σs) ≥ (Deref #[ScPtr l t] T, σt) : Φ.
+Proof.
+Admitted.
+
+Lemma sim_body_copy_local_r fs ft r r' n l tg ty s es σs σt Φ :
+  tsize ty = 1%nat →
+  r ≡ r' ⋅ res_mapsto l 1 s tg →
+  (r ⊨{n,fs,ft} (es, σs) ≥ (#[s], σt) : Φ) →
+  r ⊨{S n,fs,ft}
+    (es, σs) ≥ (Copy (Place l (Tagged tg) ty), σt)
+  : Φ.
+Proof.
+Admitted.
+
+Lemma sim_body_copy_unique_r
+  fs ft (r r': resUR) (h: heaplet) n (l: loc) tg T (s: scalar) es σs σt Φ :
+  tsize T = 1%nat →
+  tag_on_top σt l tg →
+  r ≡ r' ⋅ res_tag tg tkUnique h →
+  h !! l = Some s →
+  (r ⊨{n,fs,ft} (es, σs) ≥ (#[s], σt) : Φ : Prop) →
+  r ⊨{S n,fs,ft} (es, σs) ≥ (Copy (Place l (Tagged tg) T), σt) : Φ.
+Proof.
+Admitted.
+
+End right.
